

$$x \quad 0 \quad 1 \quad 2 \quad 3$$

$$y \quad 2 \quad 5 \quad 7 \quad 11$$

① linear

$$s_0(x) = 2 + \frac{5-2}{1-0}(x-0) \Rightarrow 2 + 3x \quad x \in [0, 1]$$

$$s_1(x) = 5 + \frac{7-5}{2-1}(x-1) \Rightarrow 5 + 2(x-1) = 5 + 2x - 2 = 2x + 3 \quad x \in [1, 2]$$

$$s_2(x) = 7 + \frac{11-7}{3-2}(x-2) \Rightarrow 7 + 4x - 8 = 4x - 1 \quad x \in [2, 3]$$

$$S(x) = \begin{cases} 2 + 3x, & x \in [0, 1] \\ 2x + 3, & x \in [1, 2] \\ 4x - 1, & x \in [2, 3] \end{cases}$$

② Quadratic

$$Q_i(x) = \frac{z_{i+1} - z_i}{2(t_{i+1} - t_i)}(x - t_i)^2 + z_i(x - t_i) + y_i$$

$$z_{i+1} = -z_i + 2 \left(\frac{y_{i+1} - y_i}{t_{i+1} - t_i} \right)$$

$$z_0 = 0$$

$$i=0$$

$$z_1 = -(0) + 2 \left(\frac{5-2}{1-0} \right) = 6$$

$$i=1$$

$$z_2 = -(6) + 2 \left(\frac{7-5}{2-1} \right) = -2$$

$$i=2$$

$$z_3 = -(-2) + 2 \left(\frac{11-7}{3-2} \right) = 10$$

$$z_0 = 0, z_1 = 6, z_2 = -2, z_3 = 10$$

$$Q_0(x) = \frac{6-0}{2(1-0)} (x-0)^2 + 0(x-0) + 2 \Rightarrow 3x^2 + 2 \quad x \in [0, 1]$$

$$Q_1(x) = \frac{-2-6}{2(2-1)} (x-1)^2 + 6(x-1) + 5 \Rightarrow -4(x-1)^2 + 6(x-1) + 5 \quad x \in [1, 2]$$

$$Q_2(x) = \frac{10 - (-2)}{2(3-2)} (x-2)^2 - 2(x-2) + 7 \Rightarrow 6(x-2)^2 - 2(x-2) + 7 \quad x \in [2, 3]$$

$$Q(x) = \begin{cases} 3x^2 + 2, & x \in [0, 1] \\ -4(x-1)^2 + 6(x-1) + 5, & x \in [1, 2] \\ 6(x-2)^2 - 2(x-2) + 7, & x \in [2, 3] \end{cases}$$

③ Cubic

$$f(x) = \frac{(x_{i+1} - x)^3}{6h} M_i + \frac{(x - x_i)^3}{6h} M_{i+1} + \frac{(x_{i+1} - x)}{h} \left(y_i - \frac{h^2}{6} M_i \right) + \frac{(x - x_i)}{h} \left(y_{i+1} - \frac{h^2}{6} M_{i+1} \right)$$

$$M_{i-1} + 4M_i + M_{i+1} = \frac{6}{h^2} (y_{i-1} - 2y_i + y_{i+1})$$

$$M_0, M_1, M_2, M_3$$

$$M_0, M_3 = 0$$

$$i=1$$

$$M_0 + 4M_1 + M_2 = \frac{6}{(1)^2} (2 - 2(5) + 7)$$

$$M_0 + 4M_1 + M_2 = -6$$

$$4M_1 + M_2 = -6$$

$$M_1 = \frac{-6 - M_2}{4}$$

$$i=2$$

$$M_1 + 4M_2 + M_3 = 6(5 - 2(7) + 11)$$

$$M_1 + 4M_2 = 12$$

$$M_2 = \frac{18}{5}$$

$$M_1 + 4\left(\frac{18}{5}\right) = 12$$

$$-\frac{6}{4} - \frac{1}{4}M_2 + 4M_2 = 12$$

$$M_1 = -\frac{12}{5}$$

$$\frac{15}{4}M_2 = \frac{27}{2}$$

$$M_0 = 0, M_1 = -12/5, M_2 = 18/5, M_3 = 0$$

(4)

$i=0$

$$f(x) = \frac{(1-x)^3}{6} (0) + \frac{(x-0)}{6} \left(-\frac{12}{5}\right) + \frac{(1-x)}{6} \left(2 - \frac{1^2}{6} (0)\right) + \frac{(x-0)}{1} \left(5 - \frac{1^2}{6} \left(-\frac{12}{5}\right)\right)$$

$$f_0(x) = -\frac{2}{5}x + 2(1-x) + \frac{27}{5}x$$

$i=1$

$$f(x) = \frac{(2-x)^3}{6} \left(-\frac{12}{5}\right) + \frac{(x-1)^3}{6} \left(\frac{18}{5}\right) + (2-x) \left(5 - \frac{1}{6} \left(-\frac{12}{5}\right)\right)$$

$$+ \frac{(x-1)}{1} \left(7 - \frac{1}{6} \left(\frac{18}{5}\right)\right)$$

$$= -\frac{2}{5}(2-x)^3 + \frac{3}{5}(x-1)^3 + \frac{27}{5}(2-x) + \frac{32}{5}(x-1)$$

$$i=2$$

(5)

$$f(x) = \frac{(3-x)^3}{6} \left(\frac{18}{5} \right) + \frac{(x-2)^3}{6} (0) + (3-x) \left(7 - \frac{1}{6} \left(\frac{18}{5} \right) \right)$$

$$+ \frac{(x-2)}{1} \left(11 - \frac{1}{6} (0) \right)$$

$$f(x) = \frac{3}{5} (3-x)^3 + \frac{32}{5} (3-x) + 11(x-2)$$

$$f(x) = \begin{cases} -\frac{2}{5}x + 2(1-x) + \frac{27}{5}x, & x \in [0, 1] \\ -\frac{2}{5}(2-x)^3 + \frac{3}{5}(x-1)^3 + \frac{27}{5}(2-x) + \frac{32}{5}(x-1), & x \in [1, 2] \\ \frac{3}{5}(3-x)^3 + \frac{32}{5}(3-x) + 11(x-2), & x \in [2, 3] \end{cases}$$